# Velocity Transformation
>[!example] Deriving the Velocity Transformations
>Consider an Object moving along the $x$-axis. We can find the velocity of the object in frame $S'$:$$u'=\frac{dx'}{dt'}$$
>We can relate these to $dx$ and $dt$ (in frame $S$)$$u'=\frac{\gamma_{v}(dx-vdt)}{\gamma_{v}(-\frac{v}{c^2}dx+dt)}$$
>We then cancel out the $\gamma_v$ and divide the numerator and denominator by $dt$$$u'=\frac{\frac{dx}{dt}-v}{-\frac{v}{c^2}\frac{dx}{dt}+1}$$
>By definition, $\frac{dx}{dt}=u$ which is the velocity in frame $S$. So$$u'=\frac{u-v}{1-\frac{uv}{c^{2}}}\quad\quad\text{and}\quad\quad u=\frac{u'+v}{1+\frac{u'v}{c^2}}$$


>[!important] All of the velocity transformation equations
>$$\begin{align*}
u_x'&=\frac{u_x-v}{1-\frac{u_xv}{c^2}}\\\\
u_y'&=\frac{u_y}{\gamma_v\left(1-\frac{u_xv}{c^2}\right)}\\\\
u_z'&=\frac{u_z}{\gamma_v\left(1-\frac{u_xv}{c^2}\right)}
\end{align*}$$

^58af0b
