We have an integral of the form $$S=\int_{x_1}^{x_2}f[y(x),y'(x),x]dx$$Notice this is an example of the [[Introduction to Variational Calculus#^b078e9|integral functional]]Suppose we denote our correct solution as $y(x)$. This means the integral $S$ evaluated for $y=y(x)$ is less than for any neighboring curve $y=Y(x)$. We write this neighboring curve as$$Y(x)=y(x)+\alpha\eta(x)$$Note that $\eta(x_1)=\eta(x_2)=0$. We then redefine the integral as $$S(\alpha)=\int_{x_1}^{x_2}f(Y,Y',x)dx=\int_{x_1}^{x_2}f(y+\alpha\eta,y'+\alpha\eta',x)dx$$This is then the traditional minimization problem from ordinary calculus. We simply differentiate with respect to $\alpha$, finding $\partial f/\partial\alpha$:
$$\frac{\partial f(y+\alpha\eta),y'+\alpha\eta',x}{\partial\alpha}=\eta\frac{\partial f}{\partial y}+\eta'\frac{\partial f}{\partial y'}$$and we then have
$$\frac{dS}{d\alpha}=\int_{x_1}^{x_2}\bigg(\eta\frac{\partial f}{\partial y}+\eta'\frac{\partial f}{\partial y'}\bigg)dx=0$$The second term can be rewritten using integration by parts:$$\int_{x_1}^{x_2}\eta'(x)\frac{\partial f}{\partial y'}dx=\bigg[\eta(x)\frac{\partial f}{\partial y'}\bigg]_{x_1}^{x_2}-\int_{x_1}^{x^2}\eta(x)\frac{d}{dx}\frac{\partial f}{\partial y'}dx$$Since $\eta$ at the endpoints is zero, the first term on the right vanishes, and we are left with the integral. Recombining this with the original integral gives us:$$\int_{x_1}^{x_2}\eta(x)\bigg(\frac{\partial f}{\partial y}-\frac{d}{dx}\frac{\partial f}{\partial y'}\bigg)dx=0$$Since this condition must be satisfied for any $\eta(x)$, so the other factor must be zero. This gives the Euler Lagrange Equation.
>[!example] Definition: The Euler-Lagrange Equation
>The Euler-Lagrange Equation is the differential equation given by
>$$\frac{\partial f}{\partial y}-\frac{d}{dx}\frac{\partial f}{\partial y'}=0$$

^ce4f09
